proofmode/tactics.v
@@ -1,7 +1,7 @@
 From iris.proofmode Require Import coq_tactics intro_patterns spec_patterns.
 From iris.algebra Require Export upred.
 From iris.proofmode Require Export notation.
-From iris.prelude Require Import stringmap.
+From iris.prelude Require Import stringmap hlist.
 
 Declare Reduction env_cbv := cbv [
   env_lookup env_fold env_lookup_delete env_delete env_app
@@ -11,6 +11,7 @@ Declare Reduction env_cbv := cbv [
   bool_eq_dec bool_rec bool_rect bool_dec eqb andb (* bool *)
   assci_eq_dec ascii_to_digits Ascii.ascii_dec Ascii.ascii_rec Ascii.ascii_rect
   string_eq_dec string_rec string_rect (* strings *)
+  himpl happly
   env_persistent env_spatial envs_persistent
   envs_lookup envs_lookup_delete envs_delete envs_app
     envs_simple_replace envs_replace envs_split envs_clear_spatial].
@@ -105,14 +106,6 @@ Local Tactic Notation "iPersistent" constr(H) :=
      apply _ || fail "iPersistent:" H ":" Q "not persistent"
     |env_cbv; reflexivity|].
 
-Tactic Notation "iDuplicate" constr(H1) "as" constr(H2) :=
-  eapply tac_duplicate with _ H1 _ H2 _; (* (i:=H1) (j:=H2) *)
-    [env_cbv; reflexivity || fail "iDuplicate:" H1 "not found"
-    |reflexivity || fail "iDuplicate:" H1 "not in persistent context"
-    |env_cbv; reflexivity || fail "iDuplicate:" H2 "not fresh"|].
-Tactic Notation "iDuplicate" "#" constr(H1) "as" constr(H2) :=
-  iPersistent H1; iDuplicate H1 as H2.
-
 Local Tactic Notation "iPure" constr(H) "as" simple_intropattern(pat) :=
   eapply tac_pure with _ H _ _ _; (* (i:=H1) *)
     [env_cbv; reflexivity || fail "iPure:" H "not found"
@@ -123,20 +116,36 @@ Local Tactic Notation "iPure" constr(H) "as" simple_intropattern(pat) :=
 Tactic Notation "iPureIntro" := apply uPred.const_intro.
 
 (** * Specialize *)
-Local Tactic Notation "iForallSpecialize" constr(H) open_constr(x) :=
-  eapply tac_forall_specialize with _ H _ _ x; (* (i:=H) (a:=x) *)
-    [env_cbv; reflexivity || fail "iSpecialize:" H "not found"
-    |env_cbv; reflexivity|].
+Record iTrm {X As} :=
+  ITrm { itrm : X ; itrm_vars : hlist As ; itrm_hyps : string }.
+Arguments ITrm {_ _} _ _ _.
 
-Tactic Notation "iSpecialize" constr (H) constr(pat) :=
+Notation "( H $! x1 .. xn )" :=
+  (ITrm H (hcons x1 .. (hcons xn hnil) ..) "") (at level 0, x1, xn at level 0).
+Notation "( H $! x1 .. xn 'with' pat )" :=
+  (ITrm H (hcons x1 .. (hcons xn hnil) ..) pat) (at level 0, x1, xn at level 0).
+Notation "( H 'with' pat )" := (ITrm H hnil pat) (at level 0).
+
+Tactic Notation "iSpecializeArgs" constr(H) open_constr(xs) :=
+  match xs with
+  | hnil => idtac
+  | _ =>
+    eapply tac_forall_specialize with _ H _ _ _ xs; (* (i:=H) (a:=x) *)
+      [env_cbv; reflexivity || fail 1 "iSpecialize:" H "not found"
+      |apply _ || fail 1 "iSpecialize:" H "not a forall of the right arity or type"
+      |env_cbv; reflexivity|]
+  end.
+
+Tactic Notation "iSpecializePat" constr(H) constr(pat) :=
   let solve_to_wand H1 :=
     let P := match goal with |- ToWand ?P _ _ => P end in
     apply _ || fail "iSpecialize:" H1 ":" P "not an implication/wand" in
   let rec go H1 pats :=
     lazymatch pats with
     | [] => idtac
+    | SForall :: ?pats => try (iSpecializeArgs H1 (hcons _ _)); go H1 pats
     | SAlways :: ?pats => iPersistent H1; go H1 pats
-    | SSplit true [] :: SAlways :: ?pats =>
+    | SAssert true [] :: SAlways :: ?pats =>
        eapply tac_specialize_domain_persistent with _ _ H1 _ _ _ _ _;
          [env_cbv; reflexivity || fail "iSpecialize:" H1 "not found"
          |solve_to_wand H1
@@ -167,167 +176,70 @@ Tactic Notation "iSpecialize" constr (H) constr(pat) :=
           apply _ || fail "iSpecialize:" Q "not persistent"
          |env_cbv; reflexivity| |go H1 pats]
     | SPure :: ?pats =>
-       eapply tac_specialize_range_persistent with _ _ H1 _ _ _ _; (* make custom tac_ lemma *)
+       eapply tac_specialize_range_persistent with _ _ H1 _ _ _ _;
+         (* make custom tac_ lemma *)
          [env_cbv; reflexivity || fail "iSpecialize:" H1 "not found"
          |solve_to_wand H1
          |let Q := match goal with |- PersistentP ?Q => Q end in
           apply _ || fail "iSpecialize:" Q "not persistent"
          |env_cbv; reflexivity|iPureIntro|go H1 pats]
-    | SSplit ?lr ?Hs :: ?pats =>
+    | SAssert ?lr ?Hs :: ?pats =>
        eapply tac_specialize_assert with _ _ _ H1 _ lr Hs _ _ _;
          [env_cbv; reflexivity || fail "iSpecialize:" H1 "not found"
          |solve_to_wand H1
          |env_cbv; reflexivity || fail "iSpecialize:" Hs "not found"|
          |go H1 pats]
-    end in
-  repeat (iForallSpecialize H _);
-  let pats := spec_pat.parse pat in go H pats.
+    end in let pats := spec_pat.parse pat in go H pats.
 
-Tactic Notation "iSpecialize" constr (H) "{" open_constr(x1) "}" :=
-  iForallSpecialize H x1.
-Tactic Notation "iSpecialize" constr (H) "{" open_constr(x1)
-    open_constr(x2) "}" :=
-  iSpecialize H { x1 }; iForallSpecialize H x2.
-Tactic Notation "iSpecialize" constr (H) "{" open_constr(x1) open_constr(x2)
-    open_constr(x3) "}" :=
-  iSpecialize H { x1 x2 }; iForallSpecialize H x3.
-Tactic Notation "iSpecialize" constr (H) "{" open_constr(x1) open_constr(x2)
-    open_constr(x3) open_constr(x4) "}" :=
-  iSpecialize H { x1 x2 x3 }; iForallSpecialize H x4.
-Tactic Notation "iSpecialize" constr (H) "{" open_constr(x1) open_constr(x2)
-     open_constr(x3) open_constr(x4) open_constr(x5) "}" :=
-  iSpecialize H { x1 x2 x3 x4 }; iForallSpecialize H x5.
-Tactic Notation "iSpecialize" constr (H) "{" open_constr(x1) open_constr(x2)
-    open_constr(x3) open_constr(x4) open_constr(x5) open_constr(x6) "}" :=
-  iSpecialize H { x1 x2 x3 x4 x5 }; iForallSpecialize H x6.
-Tactic Notation "iSpecialize" constr (H) "{" open_constr(x1) open_constr(x2)
-    open_constr(x3) open_constr(x4) open_constr(x5) open_constr(x6)
-    open_constr(x7) "}" :=
-  iSpecialize H { x1 x2 x3 x4 x5 x6 }; iForallSpecialize H x7.
-Tactic Notation "iSpecialize" constr (H) "{" open_constr(x1) open_constr(x2)
-    open_constr(x3) open_constr(x4) open_constr(x5) open_constr(x6)
-    open_constr(x7) open_constr(x8) "}" :=
-  iSpecialize H { x1 x2 x3 x4 x5 x6 x7 }; iForallSpecialize H x8.
-
-Tactic Notation "iSpecialize" constr (H) "{" open_constr(x1) "}" constr(Hs) :=
-  iSpecialize H { x1 }; iSpecialize H @ Hs.
-Tactic Notation "iSpecialize" constr (H) "{" open_constr(x1) open_constr(x2) "}"
-    constr(Hs) :=
-  iSpecialize H { x1 x2 }; iSpecialize H @ Hs.
-Tactic Notation "iSpecialize" constr (H) "{" open_constr(x1) open_constr(x2)
-    open_constr(x3) "}" constr(Hs) :=
-  iSpecialize H { x1 x2 x3 }; iSpecialize H @ Hs.
-Tactic Notation "iSpecialize" constr (H) "{" open_constr(x1) open_constr(x2)
-    open_constr(x3) open_constr(x4) "}" constr(Hs) :=
-  iSpecialize H { x1 x2 x3 x4 }; iSpecialize H @ Hs.
-Tactic Notation "iSpecialize" constr (H) "{" open_constr(x1) open_constr(x2)
-    open_constr(x3) open_constr(x4) open_constr(x5) "}" constr(Hs) :=
-  iSpecialize H { x1 x2 x3 x4 x5 }; iSpecialize H @ Hs.
-Tactic Notation "iSpecialize" constr (H) "{" open_constr(x1) open_constr(x2)
-    open_constr(x3) open_constr(x4) open_constr(x5) open_constr(x6) "}"
-    constr(Hs) :=
-  iSpecialize H { x1 x2 x3 x4 x5 x6 }; iSpecialize H @ Hs.
-Tactic Notation "iSpecialize" constr (H) "{" open_constr(x1) open_constr(x2)
-    open_constr(x3) open_constr(x4) open_constr(x5) open_constr(x6)
-    open_constr(x7) "}" constr(Hs) :=
-  iSpecialize H { x1 x2 x3 x4 x5 x6 x7 }; iSpecialize H @ Hs.
-Tactic Notation "iSpecialize" constr (H) "{" open_constr(x1) open_constr(x2)
-    open_constr(x3) open_constr(x4) open_constr(x5) open_constr(x6)
-    open_constr(x7) open_constr(x8) "}" constr(Hs) :=
-  iSpecialize H { x1 x2 x3 x4 x5 x6 x7 x8 }; iSpecialize H @ Hs.
-
-(** * Pose proof *)
-Tactic Notation "iPoseProof" open_constr(lem) "as" constr(H) :=
-  eapply tac_pose_proof with _ H _ _ _; (* (j:=H) *)
-    [first
-       [eapply lem
-       |apply uPred.equiv_iff; eapply lem]
-    |apply _
-    |env_cbv; reflexivity || fail "iPoseProof:" H "not fresh"|].
-
-Tactic Notation "iPoseProof" open_constr(lem) constr(Hs) "as" constr(H) :=
-  iPoseProof lem as H; last iSpecialize H Hs.
-
-Tactic Notation "iPoseProof" open_constr(lem) :=
-  let H := iFresh in iPoseProof lem as H.
-Tactic Notation "iPoseProof" open_constr(lem) constr(Hs) :=
-  let H := iFresh in iPoseProof lem Hs as H.
-
-Tactic Notation "iPoseProof" open_constr(lem) "as" tactic(tac) :=
-  lazymatch type of lem with
-  | string => tac lem
-  | _ => let H := iFresh in iPoseProof lem as H; last tac H; try apply _
+Tactic Notation "iSpecialize" open_constr(t) :=
+  match t with
+  | ITrm ?H ?xs ?pat => iSpecializeArgs H xs; iSpecializePat H pat
   end.
 
-Tactic Notation "iPoseProof" open_constr(lem) constr(Hs) "as" tactic(tac) :=
-  iPoseProof lem as (fun H => iSpecialize H Hs; last tac H).
+(** * Pose proof *)
+Tactic Notation "iPoseProofCore" open_constr(H1) "as" constr(H2) :=
+  lazymatch type of H1 with
+  | string =>
+     eapply tac_pose_proof_hyp with _ _ H1 _ H2 _;
+       [env_cbv; reflexivity || fail "iPoseProof:" H1 "not found"
+       |env_cbv; reflexivity || fail "iPoseProof:" H2 "not fresh"|]
+  | _ =>
+     eapply tac_pose_proof with _ H2 _ _ _; (* (j:=H) *)
+       [first [eapply H1|apply uPred.equiv_iff; eapply H1]
+       |apply _
+       |env_cbv; reflexivity || fail "iPoseProof:" H2 "not fresh"|]
+  end.
+
+Tactic Notation "iPoseProof" open_constr(t) "as" constr(H) :=
+  lazymatch t with
+  | ITrm ?H1 ?xs ?pat =>
+     iPoseProofCore H1 as H; last (iSpecializeArgs H xs; iSpecializePat H pat)
+  | _ => iPoseProofCore t as H
+  end.
+
+Tactic Notation "iPoseProof" open_constr(t) :=
+  let H := iFresh in iPoseProof t as H.
 
 (** * Apply *)
-Tactic Notation "iApply" open_constr (lem) :=
-  iPoseProof lem as (fun H => repeat (iForallSpecialize H _); first
-    [iExact H
-    |eapply tac_apply with _ H _ _ _;
-       [env_cbv; reflexivity || fail 1 "iApply:" lem "not found"
-       |apply _ || fail 1 "iApply: cannot apply" lem|]]).
-Tactic Notation "iApply" open_constr (H) "{" open_constr(x1) "}" :=
-  iSpecialize H { x1 }; last iApply H.
-Tactic Notation "iApply" open_constr (H) "{" open_constr(x1)
-    open_constr(x2) "}" :=
-  iSpecialize H { x1 x2 }; last iApply H.
-Tactic Notation "iApply" open_constr (H) "{" open_constr(x1) open_constr(x2)
-    open_constr(x3) "}" :=
-  iSpecialize H { x1 x2 x3 }; last iApply H.
-Tactic Notation "iApply" open_constr (H) "{" open_constr(x1) open_constr(x2)
-    open_constr(x3) open_constr(x4) "}" :=
-  iSpecialize H { x1 x2 x3 x4 }; last iApply H.
-Tactic Notation "iApply" open_constr (H) "{" open_constr(x1) open_constr(x2)
-     open_constr(x3) open_constr(x4) open_constr(x5) "}" :=
-  iSpecialize H { x1 x2 x3 x4 x5 }; last iApply H.
-Tactic Notation "iApply" open_constr (H) "{" open_constr(x1) open_constr(x2)
-    open_constr(x3) open_constr(x4) open_constr(x5) open_constr(x6) "}" :=
-  iSpecialize H { x1 x2 x3 x4 x5 x6 }; last iApply H.
-Tactic Notation "iApply" open_constr (H) "{" open_constr(x1) open_constr(x2)
-    open_constr(x3) open_constr(x4) open_constr(x5) open_constr(x6)
-    open_constr(x7) "}" :=
-  iSpecialize H { x1 x2 x3 x4 x5 x6 x7 }; last iApply H.
-Tactic Notation "iApply" open_constr (H) "{" open_constr(x1) open_constr(x2)
-    open_constr(x3) open_constr(x4) open_constr(x5) open_constr(x6)
-    open_constr(x7) open_constr(x8) "}" :=
-  iSpecialize H { x1 x2 x3 x4 x5 x6 x7 x8 }; last iApply H.
+Tactic Notation "iApplyCore" constr(H) := first
+  [iExact H
+  |eapply tac_apply with _ H _ _ _;
+     [env_cbv; reflexivity || fail 1 "iApply:" H "not found"
+     |apply _ || fail 1 "iApply: cannot apply" H|]].
 
-(* this is wrong *)
-Tactic Notation "iApply" open_constr (lem) constr(Hs) :=
-  iPoseProof lem Hs as (fun H => first
-    [iExact H
-    |eapply tac_apply with _ H _ _ _;
-       [env_cbv; reflexivity || fail 1 "iApply:" lem "not found"
-       |apply _ || fail 1 "iApply: cannot apply" lem|]]).
-Tactic Notation "iApply" open_constr (H) "{" open_constr(x1) "}" constr(Hs) :=
-  iSpecialize H { x1 }; last iApply H Hs.
-Tactic Notation "iApply" open_constr (H) "{" open_constr(x1) open_constr(x2) "}"
-    constr(Hs) :=
-  iSpecialize H { x1 x2 }; last iApply H Hs.
-Tactic Notation "iApply" open_constr (H) "{" open_constr(x1) open_constr(x2)
-    open_constr(x3) "}" constr(Hs) :=
-  iSpecialize H { x1 x2 x3 }; last iApply H Hs.
-Tactic Notation "iApply" open_constr (H) "{" open_constr(x1) open_constr(x2)
-    open_constr(x3) open_constr(x4) "}" constr(Hs) :=
-  iSpecialize H { x1 x2 x3 x4 }; last iApply H Hs.
-Tactic Notation "iApply" open_constr (H) "{" open_constr(x1) open_constr(x2)
-    open_constr(x3) open_constr(x4) open_constr(x5) "}" constr(Hs) :=
-  iSpecialize H { x1 x2 x3 x4 x5 }; last iApply H Hs.
-Tactic Notation "iApply" open_constr (H) "{" open_constr(x1) open_constr(x2)
-    open_constr(x3) open_constr(x4) open_constr(x5) open_constr(x6) "}"
-    constr(Hs) :=
-  iSpecialize H { x1 x2 x3 x4 x5 x6 }; last iApply H Hs.
-Tactic Notation "iApply" open_constr (H) "{" open_constr(x1) open_constr(x2)
-    open_constr(x3) open_constr(x4) open_constr(x5) open_constr(x6)
-    open_constr(x7) "}" constr(Hs) :=
-  iSpecialize H { x1 x2 x3 x4 x5 x6 x7 }; last iApply H Hs.
-Tactic Notation "iApply" open_constr (H) "{" open_constr(x1) open_constr(x2)
-    open_constr(x3) open_constr(x4) open_constr(x5) open_constr(x6)
-    open_constr(x7) open_constr(x8) "}" constr(Hs) :=
-  iSpecialize H { x1 x2 x3 x4 x5 x6 x7 x8 }; last iApply H Hs.
+Tactic Notation "iApply" open_constr(t) :=
+  let Htmp := iFresh in
+  lazymatch t with
+  | ITrm ?H ?xs ?pat =>
+     iPoseProofCore H as Htmp; last (
+       iSpecializeArgs Htmp xs;
+       try (iSpecializeArgs Htmp (hcons _ _));
+       iSpecializePat Htmp pat; last iApplyCore Htmp)
+  | _ =>
+     iPoseProofCore t as Htmp; last (
+       try (iSpecializeArgs Htmp (hcons _ _));
+       iApplyCore Htmp)
+  end; try apply _.
 
 (** * Revert *)
 Local Tactic Notation "iForallRevert" ident(x) :=
@@ -548,94 +460,59 @@ Local Tactic Notation "iDestructHyp" constr(H) "as" "{" simple_intropattern(x1)
     simple_intropattern(x8) "}" constr(pat) :=
   iExistDestruct H as x1 H; iDestructHyp H as { x2 x3 x4 x5 x6 x7 x8 } pat.
 
+Tactic Notation "iDestructHelp" open_constr(lem) "as" tactic(tac) :=
+  lazymatch type of lem with
+  | string => tac lem
+  | iTrm =>
+     lazymatch lem with
+     | @iTrm string ?H _ hnil ?pat =>
+        iSpecializePat H pat; last tac H
+     | _ => let H := iFresh in iPoseProof lem as H; last tac H; try apply _
+     end
+  | _ => let H := iFresh in iPoseProof lem as H; last tac H; try apply _
+  end.
+
 Tactic Notation "iDestruct" open_constr(H) "as" constr(pat) :=
-  iPoseProof H as (fun H => iDestructHyp H as pat).
+  iDestructHelp H as (fun H => iDestructHyp H as pat).
 Tactic Notation "iDestruct" open_constr(H) "as" "{" simple_intropattern(x1) "}"
     constr(pat) :=
-  iPoseProof H as (fun H => iDestructHyp H as { x1 } pat).
+  iDestructHelp H as (fun H => iDestructHyp H as { x1 } pat).
 Tactic Notation "iDestruct" open_constr(H) "as" "{" simple_intropattern(x1)
     simple_intropattern(x2) "}" constr(pat) :=
-  iPoseProof H as (fun H => iDestructHyp H as { x1 x2 } pat).
+  iDestructHelp H as (fun H => iDestructHyp H as { x1 x2 } pat).
 Tactic Notation "iDestruct" open_constr(H) "as" "{" simple_intropattern(x1)
     simple_intropattern(x2) simple_intropattern(x3) "}" constr(pat) :=
-  iPoseProof H as (fun H => iDestructHyp H as { x1 x2 x3 } pat).
+  iDestructHelp H as (fun H => iDestructHyp H as { x1 x2 x3 } pat).
 Tactic Notation "iDestruct" open_constr(H) "as" "{" simple_intropattern(x1)
     simple_intropattern(x2) simple_intropattern(x3) simple_intropattern(x4) "}"
     constr(pat) :=
-  iPoseProof H as (fun H => iDestructHyp H as { x1 x2 x3 x4 } pat).
+  iDestructHelp H as (fun H => iDestructHyp H as { x1 x2 x3 x4 } pat).
 Tactic Notation "iDestruct" open_constr(H) "as" "{" simple_intropattern(x1)
     simple_intropattern(x2) simple_intropattern(x3) simple_intropattern(x4)
     simple_intropattern(x5) "}" constr(pat) :=
-  iPoseProof H as (fun H => iDestructHyp H as { x1 x2 x3 x4 x5 } pat).
+  iDestructHelp H as (fun H => iDestructHyp H as { x1 x2 x3 x4 x5 } pat).
 Tactic Notation "iDestruct" open_constr(H) "as" "{" simple_intropattern(x1)
     simple_intropattern(x2) simple_intropattern(x3) simple_intropattern(x4)
     simple_intropattern(x5) simple_intropattern(x6) "}" constr(pat) :=
-  iPoseProof H as (fun H => iDestructHyp H as { x1 x2 x3 x4 x5 x6 } pat).
+  iDestructHelp H as (fun H => iDestructHyp H as { x1 x2 x3 x4 x5 x6 } pat).
 Tactic Notation "iDestruct" open_constr(H) "as" "{" simple_intropattern(x1)
     simple_intropattern(x2) simple_intropattern(x3) simple_intropattern(x4)
     simple_intropattern(x5) simple_intropattern(x6) simple_intropattern(x7) "}"
     constr(pat) :=
-  iPoseProof H as (fun H => iDestructHyp H as { x1 x2 x3 x4 x5 x6 x7 } pat).
+  iDestructHelp H as (fun H => iDestructHyp H as { x1 x2 x3 x4 x5 x6 x7 } pat).
 Tactic Notation "iDestruct" open_constr(H) "as" "{" simple_intropattern(x1)
     simple_intropattern(x2) simple_intropattern(x3) simple_intropattern(x4)
     simple_intropattern(x5) simple_intropattern(x6) simple_intropattern(x7)
     simple_intropattern(x8) "}" constr(pat) :=
-  iPoseProof H as (fun H => iDestructHyp H as { x1 x2 x3 x4 x5 x6 x7 x8 } pat).
-
-Tactic Notation "iDestruct" open_constr(lem) constr(Hs) "as" constr(pat) :=
-  iPoseProof lem as (fun H => iSpecialize H Hs; last iDestructHyp H as pat).
-Tactic Notation "iDestruct" open_constr(lem) constr(Hs) "as" "{"
-    simple_intropattern(x1) "}" constr(pat) :=
-  iPoseProof lem as (fun H => iSpecialize H Hs;
-    last iDestructHyp H as { x1 } pat).
-Tactic Notation "iDestruct" open_constr(lem) constr(Hs) "as" "{"
-    simple_intropattern(x1) simple_intropattern(x2) "}" constr(pat) :=
-  iPoseProof lem as (fun H => iSpecialize H Hs;
-    last iDestructHyp H as { x1 x2 } pat).
-Tactic Notation "iDestruct" open_constr(lem) constr(Hs) "as" "{"
-    simple_intropattern(x1) simple_intropattern(x2) simple_intropattern(x3) "}"
-    constr(pat) :=
-  iPoseProof lem as (fun H => iSpecialize H Hs;
-    last iDestructHyp H as { x1 x2 x3 } pat).
-Tactic Notation "iDestruct" open_constr(lem) constr(Hs) "as" "{"
-    simple_intropattern(x1) simple_intropattern(x2) simple_intropattern(x3)
-    simple_intropattern(x4) "}" constr(pat) :=
-  iPoseProof lem as (fun H => iSpecialize H Hs;
-    last iDestructHyp H as { x1 x2 x3 x4 } pat).
-Tactic Notation "iDestruct" open_constr(lem) constr(Hs) "as" "{"
-    simple_intropattern(x1) simple_intropattern(x2) simple_intropattern(x3)
-    simple_intropattern(x4) simple_intropattern(x5) "}" constr(pat) :=
-  iPoseProof lem as (fun H => iSpecialize H Hs;
-    last iDestructHyp H as { x1 x2 x3 x4 x5 } pat).
-Tactic Notation "iDestruct" open_constr(lem) constr(Hs) "as" "{"
-    simple_intropattern(x1) simple_intropattern(x2) simple_intropattern(x3)
-    simple_intropattern(x4) simple_intropattern(x5) simple_intropattern(x6) "}"
-    constr(pat) :=
-  iPoseProof lem as (fun H => iSpecialize H Hs;
-    last iDestructHyp H as { x1 x2 x3 x4 x5 x6 } pat).
-Tactic Notation "iDestruct" open_constr(lem) constr(Hs) "as" "{"
-    simple_intropattern(x1) simple_intropattern(x2) simple_intropattern(x3)
-    simple_intropattern(x4) simple_intropattern(x5) simple_intropattern(x6)
-    simple_intropattern(x7) "}" constr(pat) :=
-  iPoseProof lem as (fun H => iSpecialize H Hs;
-    last iDestructHyp H as { x1 x2 x3 x4 x5 x6 x7 } pat).
-Tactic Notation "iDestruct" open_constr(lem) constr(Hs) "as" "{"
-    simple_intropattern(x1) simple_intropattern(x2) simple_intropattern(x3)
-    simple_intropattern(x4) simple_intropattern(x5) simple_intropattern(x6)
-    simple_intropattern(x7) simple_intropattern(x8) "}" constr(pat) :=
-  iPoseProof lem as (fun H => iSpecialize H Hs;
-    last iDestructHyp H as { x1 x2 x3 x4 x5 x6 x7 x8 } pat).
+  iDestructHelp H as (fun H => iDestructHyp H as { x1 x2 x3 x4 x5 x6 x7 x8 } pat).
 
 Tactic Notation "iDestruct" open_constr(H) "as" "%" simple_intropattern(pat) :=
   let Htmp := iFresh in iDestruct H as Htmp; iPure Htmp as pat.
-Tactic Notation "iDestruct" open_constr(H) constr(Hs)
-    "as" "%" simple_intropattern(pat) :=
-  let Htmp := iFresh in iDestruct H Hs as Htmp; iPure Htmp as pat.
 
 (** * Always *)
 Tactic Notation "iAlways":=
-   apply tac_always_intro;
-     [reflexivity || fail "iAlways: spatial context non-empty"|].
+  apply tac_always_intro;
+    [reflexivity || fail "iAlways: spatial context non-empty"|].
 
 (** * Later *)
 Tactic Notation "iNext":=
@@ -760,7 +637,7 @@ Tactic Notation "iIntros" "{" simple_intropattern(x1) simple_intropattern(x2)
 
 (* This is pretty ugly, but without Ltac support for manipulating lists of
 idents I do not know how to do this better. *)
-Local Ltac iLöbCore IH tac_before tac_after :=
+Local Ltac iLöbHelp IH tac_before tac_after :=
   match goal with
   | |- of_envs ?Δ ⊢ _ =>
      let Hs := constr:(reverse (env_dom_list (env_spatial Δ))) in
@@ -771,31 +648,31 @@ Local Ltac iLöbCore IH tac_before tac_after :=
     tac_after; iIntros Hs
   end.
 
-Tactic Notation "iLöb" "as" constr (IH) := iLöbCore IH idtac idtac.
+Tactic Notation "iLöb" "as" constr (IH) := iLöbHelp IH idtac idtac.
 Tactic Notation "iLöb" "{" ident(x1) "}" "as" constr (IH) :=
-  iLöbCore IH ltac:(iRevert { x1 }) ltac:(iIntros { x1 }).
+  iLöbHelp IH ltac:(iRevert { x1 }) ltac:(iIntros { x1 }).
 Tactic Notation "iLöb" "{" ident(x1) ident(x2) "}" "as" constr (IH) :=
-  iLöbCore IH ltac:(iRevert { x1 x2 }) ltac:(iIntros { x1 x2 }).
+  iLöbHelp IH ltac:(iRevert { x1 x2 }) ltac:(iIntros { x1 x2 }).
 Tactic Notation "iLöb" "{" ident(x1) ident(x2) ident(x3) "}" "as" constr (IH) :=
-  iLöbCore IH ltac:(iRevert { x1 x2 x3 }) ltac:(iIntros { x1 x2 x3 }).
+  iLöbHelp IH ltac:(iRevert { x1 x2 x3 }) ltac:(iIntros { x1 x2 x3 }).
 Tactic Notation "iLöb" "{" ident(x1) ident(x2) ident(x3) ident(x4) "}" "as"
     constr (IH):=
-  iLöbCore IH ltac:(iRevert { x1 x2 x3 x4 }) ltac:(iIntros { x1 x2 x3 x4 }).
+  iLöbHelp IH ltac:(iRevert { x1 x2 x3 x4 }) ltac:(iIntros { x1 x2 x3 x4 }).
 Tactic Notation "iLöb" "{" ident(x1) ident(x2) ident(x3) ident(x4)
     ident(x5) "}" "as" constr (IH) :=
-  iLöbCore IH ltac:(iRevert { x1 x2 x3 x4 x5 })
+  iLöbHelp IH ltac:(iRevert { x1 x2 x3 x4 x5 })
               ltac:(iIntros { x1 x2 x3 x4 x5 }).
 Tactic Notation "iLöb" "{" ident(x1) ident(x2) ident(x3) ident(x4)
     ident(x5) ident(x6) "}" "as" constr (IH) :=
-  iLöbCore IH ltac:(iRevert { x1 x2 x3 x4 x5 x6 })
+  iLöbHelp IH ltac:(iRevert { x1 x2 x3 x4 x5 x6 })
               ltac:(iIntros { x1 x2 x3 x4 x5 x6 }).
 Tactic Notation "iLöb" "{" ident(x1) ident(x2) ident(x3) ident(x4)
     ident(x5) ident(x6) ident(x7) "}" "as" constr (IH) :=
-  iLöbCore IH ltac:(iRevert { x1 x2 x3 x4 x5 x6 x7 })
+  iLöbHelp IH ltac:(iRevert { x1 x2 x3 x4 x5 x6 x7 })
               ltac:(iIntros { x1 x2 x3 x4 x5 x6 x7 }).
 Tactic Notation "iLöb" "{" ident(x1) ident(x2) ident(x3) ident(x4)
     ident(x5) ident(x6) ident(x7) ident(x8) "}" "as" constr (IH) :=
-  iLöbCore IH ltac:(iRevert { x1 x2 x3 x4 x5 x6 x7 x8 })
+  iLöbHelp IH ltac:(iRevert { x1 x2 x3 x4 x5 x6 x7 x8 })
               ltac:(iIntros { x1 x2 x3 x4 x5 x6 x7 x8 }).
 
 (** * Assert *)
@@ -803,7 +680,7 @@ Tactic Notation "iAssert" constr(Q) "as" constr(pat) "with" constr(Hs) :=
   let H := iFresh in
   let Hs := spec_pat.parse_one Hs in
   lazymatch Hs with
-  | SSplit ?lr ?Hs =>
+  | SAssert ?lr ?Hs =>
      eapply tac_assert with _ _ _ lr Hs H Q; (* (js:=Hs) (j:=H) (P:=Q) *)
        [env_cbv; reflexivity || fail "iAssert:" Hs "not found"
        |env_cbv; reflexivity|
